alternative specs

crdt_specs2.thy
@@ -17,18 +17,30 @@ type_synonym ('op, 'opn, 'res) ccrdtSpec =
       \<Rightarrow> (callId \<Rightarrow>'op)              \<comment> \<open>call information\<close> 
       \<Rightarrow> callId rel                  \<comment> \<open>happens-before\<close>
       \<Rightarrow> ('opn \<Rightarrow> 'op)               \<comment> \<open>mapping back\<close>
-      \<Rightarrow> 'op 
+      \<Rightarrow> 'opn 
       \<Rightarrow> 'res
       \<Rightarrow> bool"
 
 text "There is a mapping between the composable CRDT specs above and the original specifications:"
 
-(* TODO *)
+(* TODO
+so far the relation is only without nesting (for identity mapping.
+Must add the mapping to both sides of the equation
+left through transforming the context, right through C directly
+
+best to prove equivalence for the map first and see what is required
+ *)
+definition crdt_spec_rel :: "('op, 'res) crdtSpec \<Rightarrow> ('op, 'op, 'res) ccrdtSpec \<Rightarrow> bool" where
+"crdt_spec_rel spec cspec \<equiv>
+(\<forall>ctxt op r. 
+spec op ctxt r \<longleftrightarrow> cspec (dom (calls ctxt)) (\<lambda>c. case calls ctxt c of Some (Call op r) \<Rightarrow> op) (happensBefore ctxt) id op r)
+
+"
 
 
 subsection "Register"
 
-definition 
+definition latest_assignments' :: "callId set \<Rightarrow> (callId \<Rightarrow> 'op) \<Rightarrow> (callId \<times> callId) set \<Rightarrow> ('v registerOp \<Rightarrow> 'op) \<Rightarrow> (callId \<times> 'v) set"  where
 "latest_assignments' vis op hb C \<equiv> 
    {(c,v). c\<in>vis \<and> op c = C (Assign v) \<and> (\<nexists>c' v'. c'\<in>vis \<and> op c' = C (Assign v') \<and> (c,c')\<in>hb)}"
 
@@ -50,13 +62,84 @@ definition firstValue' :: "'a \<Rightarrow> ('b \<times> 'a) set \<Rightarrow> '
   "
 
 
-definition 
+definition lww_register_spec' :: "('v::default) \<Rightarrow> ('op, 'v registerOp, 'v) ccrdtSpec" where
 "lww_register_spec' initial vis op hb C oper res \<equiv> 
   case oper of
     Assign x \<Rightarrow> res = default
-  | Read \<Rightarrow> res = firstValue' initial (latest_values' vis op hb C)"
+  | Read \<Rightarrow> res = firstValue' initial (latest_assignments' vis op hb C)"
 
 
+lemma 
+"crdt_spec_rel (lww_register_spec initial) (lww_register_spec' initial) "
+  unfolding crdt_spec_rel_def
+proof (intro allI impI)
+
+  show "lww_register_spec initial op ctxt r =
+       lww_register_spec' initial (dom (calls ctxt)) (\<lambda>c. case calls ctxt c of None \<Rightarrow> ??? | Some (Call op r) \<Rightarrow> op) (happensBefore ctxt)
+        id op r" (is ?g)
+    for ctxt op r
+  proof -
+
+    have h1: "(latest_assignments' (dom (calls ctxt)) (\<lambda>c. case calls ctxt c of None \<Rightarrow> ??? | Some (Call op r) \<Rightarrow> op) (happensBefore ctxt) id)
+    = {(x,y). latestAssignments ctxt x \<triangleq> y}"
+      apply (auto simp add: latest_assignments'_def latestAssignments_def latestAssignments_h_def split: call.splits)
+         apply (auto split: option.splits call.splits registerOp.splits if_splits)
+      done
+
+    have h2: "(fst ` {(x, y). latestAssignments ctxt x \<triangleq> y}) =
+              (dom (latestAssignments ctxt))"
+      by (auto simp add: in_img_simp)
+
+
+    have h3: "firstValue' initial {(x, y). latestAssignments ctxt x \<triangleq> y}
+          = firstValue initial (latestAssignments ctxt)"
+      apply (auto simp add: firstValue'_def firstValue_def h2)
+      by (smt dom_def emptyE mem_Collect_eq option.exhaust option.sel some_well_order_includes_all some_well_order_is_wo_rel wo_rel.minim_in)
+
+
+
+    show ?g
+      apply (auto simp add: lww_register_spec_def lww_register_spec'_def split: registerOp.splits)
+      apply (auto simp add: h1 h3)
+      done
+  qed
+qed
+
+
+
+
+subsection "Sets"
+
+definition set_rw_spec' where
+"set_rw_spec' from_bool vis op hb C oper res \<equiv> 
+  case oper of
+    Add _ => res = default
+  | Remove _ \<Rightarrow> res = default
+  | Contains v \<Rightarrow> res = from_bool 
+        (\<exists>a\<in>vis. a \<triangleq> Add v 
+           \<and> (\<forall>r\<in>vis. op r \<triangleq> Remove v
+                 \<longrightarrow> (\<exists>a'\<in>vis. op a' \<triangleq> Add v \<and> (r,a')\<in>hb)))"
+
+
+
+subsection "Maps"
+
+
+definition
+"deleted_calls_dw' vis op hb C k \<equiv> {c. \<exists>d\<in>vis. op d \<triangleq> C (DeleteKey k) \<and> (d,c)\<notin>hb}"
+
+definition 
+"restrict_calls vis op C k \<equiv>
+{c\<in>vis. \<exists>u. op c = C (NestedOp k u) }"
+
+definition
+"map_spec' deleted_calls from_bool nestedSpec vis op hb C oper res \<equiv>
+  case oper of
+    DeleteKey k \<Rightarrow> res = default
+  | KeyExists k \<Rightarrow> res = from_bool (\<exists>c\<in>vis. \<exists>upd_op. op c \<triangleq> NestedOp k upd_op \<and> is_update upd_op \<and>  c \<notin> deleted_calls vis op hb C k)
+  | NestedOp k nested_op \<Rightarrow>
+     nestedSpec (restrict_calls vis op C k - deleted_calls vis op hb C k) op hb (\<lambda>x. C (NestedOp k x)) nested_op res
+"
 (* Needed for example: structs, set_rw, map_rw *)
 
 end
